lakefile.lean
@@ -24,4 +24,5 @@ lean_lib Generated where
 @[default_target]
 lean_lib Examples where
   roots := #[`Examples.MaxProof, `Examples.MetaMTest, `Examples.Benchmark,
-             `Examples.GcdProof, `Examples.GcdCorrect]
+             `Examples.GcdProof, `Examples.GcdCorrect, `Examples.GcdTypeStrengthen,
+             `Examples.GcdWordAbstract, `Examples.GcdPhase2]
